src/promotion/iSimThreadOther.v
@@ -78,9 +78,9 @@ Module SimThreadOther.
     - econs 2. econs; eauto.
     - inv SIM1. ss. econs; eauto; ss.
       i. inv STEP_SRC.
-      erewrite <- promise_eq_promises; try exact PROMISE; eauto.
+      erewrite Memory.promise_get_diff_promise; try exact PROMISE; eauto. 
     - i. s. inv STEP_SRC.
-      erewrite promise_eq_mem; try exact PROMISE; eauto.
+      erewrite <- Memory.promise_get_diff; try exact PROMISE; eauto.
   Qed.
 
   Lemma sim_thread_program_step
@@ -113,11 +113,11 @@ Module SimThreadOther.
     - econs; eauto.
       + s. eapply step_loc_free; eauto.
         inv SIM1. ss. subst. ss.
-      + s. i. inv SIM1.
-        erewrite <- program_step_eq_promises; eauto.
+      + s. i. inv SIM1. ss.
+        erewrite <- Local.program_step_get_diff_promises; eauto.
         erewrite ThreadEvent.eq_program_event_eq_loc; eauto.
     - s. i.
-      eapply program_step_eq_mem; eauto.
+      eapply Local.program_step_get_diff; eauto.
       erewrite ThreadEvent.eq_program_event_eq_loc; eauto.
   Qed.
 
@@ -213,7 +213,7 @@ Module SimThreadOther.
 
   Lemma sim_thread_plus_step
         l e1_src
-        pf e_tgt e1_tgt e2_tgt e3_tgt
+        e_tgt e1_tgt e2_tgt e3_tgt
         (SIM1: sim_thread l e1_src e1_tgt)
         (WF1_SRC: Local.wf (Thread.local e1_src) (Thread.memory e1_src))
         (WF1_TGT: Local.wf (Thread.local e1_tgt) (Thread.memory e1_tgt))
@@ -222,7 +222,7 @@ Module SimThreadOther.
         (CLOSED1_SRC: Memory.closed (Thread.memory e1_src))
         (CLOSED1_TGT: Memory.closed (Thread.memory e1_tgt))
         (STEPS_TGT: rtc (@Thread.tau_step (lang R)) e1_tgt e2_tgt)
-        (STEP_TGT: Thread.step pf e_tgt e2_tgt e3_tgt):
+        (STEP_TGT: Thread.opt_step e_tgt e2_tgt e3_tgt):
     exists e_src e2_src e3_src,
       <<STEPS_SRC: rtc (@Thread.tau_step (lang R)) e1_src e2_src>> /\
       <<STEP_SRC: Thread.opt_step e_src e2_src e3_src>> /\
@@ -233,7 +233,7 @@ Module SimThreadOther.
     exploit sim_thread_rtc_tau_step; eauto. i. des.
     exploit Thread.rtc_tau_step_future; try exact STEPS_SRC; eauto. i. des.
     exploit Thread.rtc_tau_step_future; try exact STEPS_TGT; eauto. i. des.
-    exploit sim_thread_step; eauto. i. des.
+    exploit sim_thread_opt_step; eauto. i. des.
     esplits; eauto.
     i. rewrite MEMLOC. ss.
   Qed.
@@ -260,12 +260,14 @@ Module SimThreadOther.
     inv SIM1. ss. econs; s; eauto. ii.
     exploit FULFILLABLE; eauto. i. des. split; ss.
     unfold prev_released_le_loc in *. des_ifs; ss.
-    - exploit Memory.future_get1; try exact Heq0; eauto. i. des.
+    - exploit Memory.future_get1; try exact Heq0; eauto; ss. i. des.
       inv MSG_LE. inv RELEASED; try congr.
       rewrite Heq in *. inv GET.
       unnw. etrans; eauto. split; apply LE.
-    - exploit Memory.future_get1; try exact Heq0; eauto. i. des.
+    - exploit Memory.future_get1; try exact Heq0; eauto; ss. i. des.
       inv MSG_LE. inv RELEASED; try congr.
+    - exploit Memory.future_get1; try exact Heq0; eauto; ss. i. des.
+      rewrite GET in *. inv Heq. inv MSG_LE.
     - inv WF1_SRC. exploit PROMISES0; eauto. i.
       exploit PREV; eauto; ss. ii. congr.
     - inv WF1_SRC. exploit PROMISES0; eauto. i.
@@ -303,24 +305,20 @@ Module SimThreadOther.
 
   Lemma sim_thread_cap
         l e_src e_tgt
-        sc_src sc_tgt
         cap_src cap_tgt
         (SIM: sim_thread l e_src e_tgt)
         (WF_SRC: Local.wf (Thread.local e_src) (Thread.memory e_src))
         (WF_TGT: Local.wf (Thread.local e_tgt) (Thread.memory e_tgt))
         (CLOSED_SRC: Memory.closed (Thread.memory e_src))
         (CLOSED_TGT: Memory.closed (Thread.memory e_tgt))
-        (SC_SRC: Memory.max_concrete_timemap cap_src sc_src)
-        (SC_TGT: Memory.max_concrete_timemap cap_tgt sc_tgt)
         (CAP_SRC: Memory.cap (Thread.memory e_src) cap_src)
         (CAP_TGT: Memory.cap (Thread.memory e_tgt) cap_tgt):
     sim_thread l
-               (Thread.mk (lang R) (Thread.state e_src) (Thread.local e_src) sc_src cap_src)
-               (Thread.mk (lang R) (Thread.state e_tgt) (Thread.local e_tgt) sc_tgt cap_tgt).
+               (Thread.mk (lang R) (Thread.state e_src) (Thread.local e_src) (Thread.sc e_src) cap_src)
+               (Thread.mk (lang R) (Thread.state e_tgt) (Thread.local e_tgt) (Thread.sc e_tgt) cap_tgt).
   Proof.
     inv SIM. inv LOCAL.
     exploit sim_memory_cap; try exact MEMORY; eauto. i. des.
-    hexploit sim_memory_max_concrete_timemap; try exact x0; eauto. i. des.
     econs; eauto.
     s. eapply cap_fulfillable; eauto. apply WF_SRC.
   Qed.
@@ -338,22 +336,22 @@ Module SimThreadOther.
     <<CONSISTENT_SRC: Thread.consistent e_src>>.
   Proof.
     exploit Memory.cap_exists; try exact CLOSED_TGT. i. des.
-    exploit Memory.cap_closed; eauto. i.
-    exploit Memory.max_concrete_timemap_exists; try apply x0. i. des.
-    ii.
+    exploit Memory.cap_closed; eauto. ii.
     exploit sim_thread_cap; try exact SIM; try exact CAP0; try exact CAP; eauto. i.
     exploit Local.cap_wf; try exact WF_SRC; eauto. intro WF_CAP_SRC.
     exploit Local.cap_wf; try exact WF_TGT; eauto. intro WF_CAP_TGT.
-    hexploit Memory.max_concrete_timemap_closed; try exact SC_MAX. intro SC_MAX_SRC.
-    hexploit Memory.max_concrete_timemap_closed; try exact x1. intro SC_MAX_TGT.
+    hexploit Memory.cap_closed_timemap; try exact SC_SRC; eauto. i.
+    hexploit Memory.cap_closed_timemap; try exact SC_TGT; eauto. i.
     exploit Memory.cap_closed; try exact CLOSED_SRC; eauto. intro CLOSED_CAP_SRC.
     exploit Memory.cap_closed; try exact CLOSED_TGT; eauto. intro CLOSED_CAP_TGT.
     exploit CONSISTENT_TGT; eauto. i. des.
     - left. unfold Thread.steps_failure in *. des.
-      exploit sim_thread_plus_step; eauto. s. i. des.
-      destruct e_src0; ss. inv STEP_SRC.
-      destruct pf; try by (inv STEP; inv STEP0).
-      esplits; eauto.
+      exploit sim_thread_plus_step; eauto.
+      { econs 2; eauto. }
+      s. i. des.
+      inv STEP_SRC; ss; try congr.
+      destruct pf; try by (inv STEP; inv STEP0; ss; congr).
+      esplits; eauto. congr.
     - right.
       exploit sim_thread_rtc_tau_step; try exact STEPS; eauto. i. des.
       esplits; eauto.
